theories/ftlr/AddSubLt.v
@@ -27,6 +27,7 @@ Section fundamental.
     → (decodeInstrWL lw = Add dst r1 r2 \/
        decodeInstrWL lw = Sub dst r1 r2 \/
        decodeInstrWL lw = Mod dst r1 r2 \/
+       decodeInstrWL lw = HashConcat dst r1 r2 \/
        decodeInstrWL lw = Lt dst r1 r2)
     -> (□ ▷ (∀ lregs' p' b' e' a' v',
              full_map lregs'
