theories/ftlr/Hash.v
@@ -1,0 +1,54 @@
+From iris.proofmode Require Import proofmode.
+From iris.program_logic Require Import weakestpre adequacy lifting.
+From stdpp Require Import base.
+From cap_machine Require Export logrel.
+From cap_machine.ftlr Require Export ftlr_base.
+From cap_machine.rules Require Export rules_Hash rules_base.
+From cap_machine Require Import stdpp_extra.
+
+Section fundamental.
+  Context {Σ:gFunctors} {ceriseg:ceriseG Σ} {sealsg: sealStoreG Σ}
+          {nainv: logrel_na_invs Σ}
+          `{MachineParameters}.
+
+  Notation D := ((leibnizO LWord) -n> iPropO Σ).
+  Notation R := ((leibnizO LReg) -n> iPropO Σ).
+  Implicit Types lw : (leibnizO LWord).
+  Implicit Types interp : (D).
+
+  Lemma hash_case (lregs : leibnizO LReg)
+    (p : Perm) (b e a : Addr) (v : Version)
+    (lw : LWord) (dst src : RegName)  (P:D) :
+    ftlr_instr lregs p b e a v lw (Hash dst src) P.
+  Proof.
+    (* intros Hp Hsome i Hbae Hi. *)
+    (* iIntros "#IH #Hinv #Hinva #Hreg #[Hread Hwrite] Hown Ha HP Hcls HPC Hmap". *)
+    (* rewrite delete_insert_delete. *)
+    (* iDestruct ((big_sepM_delete _ _ PC) with "[HPC Hmap]") as "Hmap /="; *)
+    (*   [apply lookup_insert|rewrite delete_insert_delete;iFrame|]. simpl. *)
+    (* iApply (wp_Hash with "[$Ha $Hmap]"); eauto. *)
+    (* { by simplify_map_eq. } *)
+    (* { rewrite /subseteq /map_subseteq /set_subseteq_instance. intros rr _. *)
+    (*   apply elem_of_dom. apply lookup_insert_is_Some'; eauto. } *)
+
+    (* iIntros "!>" (regs' retv). iDestruct 1 as (HSpec) "[Ha Hmap]". *)
+    (* destruct HSpec; cycle 1. *)
+    (* { iApply wp_pure_step_later; auto. iMod ("Hcls" with "[HP Ha]");[iExists lw;iFrame|iModIntro]. iNext. *)
+    (*   iIntros "_". *)
+    (*   iApply wp_value; auto. iIntros; discriminate. } *)
+    (* { incrementLPC_inv; simplify_map_eq. *)
+    (*   iApply wp_pure_step_later; auto. iMod ("Hcls" with "[HP Ha]");[iExists lw;iFrame|iModIntro]. iNext. *)
+    (*   iIntros "_". *)
+    (*   assert (dst <> PC) as HdstPC by (intros ->; by simplify_map_eq). *)
+    (*   simplify_map_eq. *)
+    (*   iApply ("IH" $! (<[dst := _]> (<[PC := _]> lregs)) with "[%] [] [Hmap] [$Hown]"); *)
+    (*     try iClear "IH"; eauto. *)
+    (*   { intro. cbn. by repeat (rewrite lookup_insert_is_Some'; right). } *)
+    (*   iIntros (ri v Hri Hsv). *)
+    (*   rewrite insert_commute // lookup_insert_ne // in Hsv; []. *)
+    (*   destruct (decide (ri = dst)); simplify_map_eq. *)
+    (*   { repeat rewrite fixpoint_interp1_eq; auto. } *)
+    (*   { by iApply "Hreg". } rewrite !fixpoint_interp1_eq /=. destruct Hp as [-> | ->];iFrame "Hinv". } *)
+  Admitted.
+
+End fundamental.
