theories/rules/rules_AddSubLt.v
@@ -25,6 +25,7 @@ Section cap_lang_rules.
     | Sub _ _ _ => (n1 - n2)%Z
     | Mod _ _ _ => (n1 `mod` n2)%Z
     | Lt _ _ _ => (Z.b2z (n1 <? n2)%Z)
+    | HashConcat _ _ _ => (hash_concat n1 n2)
     | _ => 0%Z
     end.
 
@@ -32,6 +33,7 @@ Section cap_lang_rules.
     i = Add r arg1 arg2 ∨
     i = Sub r arg1 arg2 ∨
     i = Mod r arg1 arg2 ∨
+    i = HashConcat r arg1 arg2 ∨
     i = Lt r arg1 arg2.
 
   Lemma exec_AddSubLt_eq {i r arg1 arg2 φ} :
@@ -40,7 +42,7 @@ Section cap_lang_rules.
                    z2 ← z_of_argument (reg φ) arg2 ;
                    updatePC (update_reg φ r (WInt (denote i z1 z2))).
   Proof.
-    destruct 1 as [-> | [-> | [-> | ->] ]]; done.
+    destruct 1 as [-> | [-> | [-> | [-> | ->] ] ]]; done.
   Qed.
 
 
@@ -586,8 +588,12 @@ Proof. intros; unfold is_AddSubLt; eauto. Qed.
 Lemma is_AddSubLt_Mod dst arg1 arg2 :
   is_AddSubLt (Mod dst arg1 arg2) dst arg1 arg2.
 Proof. intros; unfold is_AddSubLt; eauto. Qed.
+Lemma is_AddSubLt_HashConcat dst arg1 arg2 :
+  is_AddSubLt (HashConcat dst arg1 arg2) dst arg1 arg2.
+Proof. intros; unfold is_AddSubLt; eauto. Qed.
 
 Global Hint Resolve is_AddSubLt_Add : core.
 Global Hint Resolve is_AddSubLt_Sub : core.
 Global Hint Resolve is_AddSubLt_Lt : core.
 Global Hint Resolve is_AddSubLt_Mod : core.
+Global Hint Resolve is_AddSubLt_HashConcat : core.
